Separate bignum spec from impl, add GM tests

code/experimental/he/Hacl.Test.HE.fst
@@ -6,13 +6,13 @@ open FStar.HyperStack.ST
 open FStar.Mul
 
 open Lib.IntTypes
+open Lib.Math.Algebra
 open Lib.Buffer
 
-open Hacl.Impl.HE.GM
-open Hacl.Impl.Bignum.Core
-open Hacl.Impl.Bignum.Convert
-open Hacl.Impl.Bignum.Comparison
-open Hacl.Impl.Bignum.Addition
+module GM = Hacl.Impl.HE.GM
+module GMS = Hacl.Spec.HE.GM
+
+open Hacl.Impl.Bignum
 
 module B = FStar.Bytes
 
@@ -30,54 +30,144 @@ val print_bool: b:bool -> ST unit (requires fun _ -> true) (ensures fun h0 _ h1 
 let print_bool b =
   C.String.print (if b then C.String.of_literal "true\n" else C.String.of_literal "false\n")
 
-val test1: unit -> Stack unit (requires fun _ -> true) (ensures fun _ _ _ -> true)
-let test1 _ =
-  push_frame();
-  //let nat1:nat = 123456781234567812345678 in
-  let list1:lbignum 1ul = nat_to_bignum_exact 100 in
-  let list2:lbignum 1ul = nat_to_bignum_exact 200 in
-  let list3:lbignum 1ul = nat_to_bignum_exact 0 in
-  let list4:lbignum 1ul = nat_to_bignum_exact 299 in
-  let list5:lbignum 1ul = nat_to_bignum_exact 300 in
 
-  print_strln "Both should be true:";
+#reset-options "--z3rlimit 50 --max_fuel 0 --max_ifuel 0"
 
-  let _ = bn_add list1 list2 list3 in
-  let res = bn_is_less list4 list3 in
-  print_bool (res = true);
+noextract inline_for_extraction
+val run_test_gm:
+     p:snat
+  -> q:snat
+  -> y:snat{y < p * q} // /\ GMS.is_nonsqr (to_fe #p y) /\ GMS.is_nonsqr (to_fe #q y)}
+  -> r:snat{r < p * q} // /\ sqr r > 0 /\ sqr r *% y > 0}
+  -> Stack unit (requires fun _ -> true) (ensures fun _ _ _ -> true)
+let run_test_gm p q y r =
 
-  let _ = bn_add list1 list2 list3 in
-  let res = bn_is_less list5 list3 in
-  print_bool (res = false);
+  push_frame ();
 
-  pop_frame()
+  assume(issnat (p*q));
 
-val test2: unit -> Stack unit (requires fun _ -> true) (ensures fun _ _ _ -> true)
-let test2 _ =
-  push_frame();
-  //let nat1:nat = 123456781234567812345678 in
-  let list1:lbignum 2ul = nat_to_bignum_exact 100000000000000000000 in
-  let list2:lbignum 2ul = nat_to_bignum_exact 200000000000000000000 in
-  let list3:lbignum 2ul = nat_to_bignum_exact 200000000000000000000 in
-  let list4:lbignum 2ul = nat_to_bignum_exact 299000000000000000000 in
-  let list5:lbignum 2ul = nat_to_bignum_exact 300000000000000000000 in
+  let aLen = nat_bytes_num p in
+  let nLen = nat_bytes_num (normalize_term (p * q)) in
 
-  print_strln "Both should be true:";
+  assume (p <= p * q);
+  assume (p-1 <= p * q);
+  snat_order (p-1) (p*q);
+  assume ((p-1)/2 <= p * q);
+  assume (issnat ((p-1)/2));
+  snat_order y (p*q);
+  snat_order r (p*q);
 
-  let _ = bn_add list1 list2 list3 in
-  let res = bn_is_less list4 list3 in
-  print_bool (res = true);
+  nat_bytes_num_fit p (p * q);
+  nat_bytes_num_fit (p-1) (p * q);
+  nat_bytes_num_fit ((p-1)/2) (p * q);
+  nat_bytes_num_fit y (p * q);
+  nat_bytes_num_fit r (p * q);
 
-  let _ = bn_add list1 list2 list3 in
-  let res = bn_is_less list5 list3 in
-  print_bool (res = false);
+  let bn_p: lbignum nLen = nat_to_bignum p in
+  let bn_p_min_one: lbignum nLen = nat_to_bignum (normalize_term (p-1)) in
+  let bn_p_min_one_half: lbignum nLen = nat_to_bignum (normalize_term ((p-1)/2)) in
+  let bn_n: lbignum nLen = nat_to_bignum (p * q) in
+  let bn_y: lbignum nLen = nat_to_bignum y in
+  let bn_r: lbignum nLen = nat_to_bignum r in
 
-  pop_frame()
+  let bn_res: lbignum nLen = create nLen (uint 0) in
+
+
+  [@inline_let]
+  let encdec (m:bool) = begin
+    print_str "\n* ";
+    print_bool m;
+
+    admit();
+
+    print_str " --enc-> ";
+    GM.encrypt bn_n bn_y bn_r m bn_res;
+    print_lbignum bn_res;
+
+    print_str " --dec-> ";
+    let m' = GM.decrypt bn_p bn_p_min_one bn_p_min_one_half bn_res in
+    print_bool m';
+
+    if (m <> m')
+      then print_str " -------------------ERROR-------------------- "
+
+    end in
+
+  encdec false;
+  encdec true;
+
+  pop_frame ()
+
+#reset-options "--z3rlimit 80 --max_fuel 2 --max_ifuel 0"
+
+val test_gm: unit -> Stack unit (requires fun _ -> true) (ensures fun _ _ _ -> true)
+let test_gm _ =
+  run_test_gm 11 7 6 6;
+  run_test_gm 5651 2309 6283665 1642087;
+
+  // 50
+  run_test_gm
+    20597963
+    18691103
+    343410843161354
+    340075475890885;
+
+  // 64
+  run_test_gm
+    3339502961
+    2462727887
+    5233939904127998699
+    5453821191296830610;
+
+  admit();
+
+  // 70
+  run_test_gm
+    21858784247
+    32600809193
+    512995630928471546296
+    451304102026366696740;
+
+  // 128
+  run_test_gm
+    15296422180258244633
+    12754350346597149907
+    135123782558807105107086847009983923035
+    119073235221716701476761821036809466296;
+
+  run_test_gm
+    18151637450909672231
+    10616931758931658067
+    169050918734026862244039761501457849989
+    91361904391308264608300641010053460290;
+
+  // 256
+  run_test_gm
+    238473831066240814685652387118826838089
+    290648921680117623622749944527302685873
+    32013853695008913941056224288699542908291901709435433477498753524425728431750
+    63966125980329819543482417151170152183116886231068453106873450906088222129050;
+
+  run_test_gm
+    194765719344750645857941111613304160759
+    302733760975917402491754353701153586917
+    36830922521294348053145663043410070557977339755323583180621317301257147794374
+    38906304989221746651998721090989108342763029754317070464956436172556984570693;
+
+  // 512
+  run_test_gm
+    90510865981466947031172959353875014846064298911390400886217098789271538551427
+    94759749888656405390748215772985529397008982247431702017685434161096778423291
+    6957432786230211466554402636790564852662237428639281229711989467622229675175469764873854713058879492065775330287649969064318829928153493172958199579400717
+    3800489529524826596462562393348890150013178998377931017956373178205920735905956480999317129649722635695766704356317847688521776746429718426269611327586578;
+
+  run_test_gm
+    110442173640700605426196791722267254977399536629395286731142679095037450319701
+    107170879681249637364506109018099376672037419626449999045129249789288431466407
+    5265437392983486448329400301105635940895238995769880107866207131125580962646642150752609876247622793613398654879743905973229074059422443151910948419853421
+    6845701554537301024323205582879742602167364769512355740049645018047271023281212094546788123698331656722332722329506942184730828849998076233448302042099044
 
 val main: unit -> St C.exit_code
 let main () =
-  print_strln "\n====== Sample: ======";
-  test1 ();
-  test2 ();
-  print_strln "=====================";
+  test_gm ();
   C.EXIT_SUCCESS
